cogent/examples/cpp2022-artefact/loops/CogentTypingHelper.thy
@@ -7,28 +7,35 @@ section "Typing helpers"
 subsection "Cogent functions"
 
 lemma typing_mono_app_cogent_fun:
-  "\<Xi>', [], [option.Some a] \<turnstile> f : b \<Longrightarrow> \<Xi>', [], [option.Some a] \<turnstile> App (Fun f []) (Var 0) : b"
+  "\<Xi>', 0, [], {}, [option.Some a] \<turnstile> f : b \<Longrightarrow> 
+   \<Xi>', 0, [], {}, [option.Some a] \<turnstile> App (Fun f [] []) (Var 0) : b"
   apply (frule typing_to_kinding_env(1); simp?)
-  apply (rule typing_app[where x = a and y = b and ?\<Gamma>1.0 = "[option.None]" and ?\<Gamma>2.0 = "[option.Some a]"]; simp?)
-    apply (clarsimp simp: split_conv_all_nth)
+  apply (rule typing_app[where x = a and y = b and 
+                ?\<Gamma>1.0 = "[option.None]" and ?\<Gamma>2.0 = "[option.Some a]"]; simp?)
+    apply (clarsimp simp: split_conv_all_nth )
     apply (rule right; simp)
-    apply (rule typing_fun[where ts = "[]", OF _ _ _ _]; (simp add: Cogent.empty_def weakening_conv_all_nth)?)
-   apply (rule none)
+   apply (rule typing_fun[where \<delta> = "[]", OF  _  _]; 
+        (simp add: Cogent.empty_def weakening_conv_all_nth)?)
+     apply (rule none, simp, simp add: subst_wellformed_nothing) 
   apply (rule typing_var; simp add: Cogent.empty_def weakening_conv_all_nth)
   apply (rule keep; simp)
   done
 
 lemma typing_mono_fun_cogent_fun:
-  "\<Xi>', [], [option.Some a] \<turnstile> f : b \<Longrightarrow> \<Xi>', [], [option.None] \<turnstile> Fun f [] : TFun a b"
+  "\<Xi>', 0, [], {}, [option.Some a] \<turnstile> f : b \<Longrightarrow> 
+   \<Xi>', 0, [], {}, [option.None] \<turnstile> Fun f [] [] : TFun a b"
   apply (frule typing_to_kinding_env(1); simp?)
-  apply (rule typing_fun[where ts = "[]", OF _ _ _ _]; (simp add: Cogent.empty_def weakening_conv_all_nth)?)
-  apply (rule none)
+  apply (rule typing_fun[where \<delta> = "[]"]; 
+        (simp add: Cogent.empty_def weakening_conv_all_nth)?)
+    apply (rule none, simp, simp add: subst_wellformed_nothing)
   done
 
 lemma typing_mono_fun_imp_appfun:
-  "\<Xi>', [], [option.None] \<turnstile> Fun f [] : TFun a b \<Longrightarrow> \<Xi>', [], [option.Some a] \<turnstile> App (Fun f []) (Var 0) : b"
+  "\<Xi>', 0, [], {}, [option.None] \<turnstile> Fun f [] []: TFun a b \<Longrightarrow> 
+   \<Xi>', 0, [], {}, [option.Some a] \<turnstile> App (Fun f [][]) (Var 0) : b"
   apply (frule typing_to_wellformed(1))
-  apply (rule typing_app[where x = a and y = b and ?\<Gamma>1.0 = "[option.None]" and ?\<Gamma>2.0 = "[option.Some a]"]; simp?)
+  apply (rule typing_app[where x = a and y = b and 
+          ?\<Gamma>1.0 = "[option.None]" and ?\<Gamma>2.0 = "[option.Some a]"]; simp?)
    apply (clarsimp simp: split_conv_all_nth)
    apply (rule right; simp)
   apply (rule typing_var; simp add: Cogent.empty_def weakening_conv_all_nth)
@@ -38,30 +45,33 @@ lemma typing_mono_fun_imp_appfun:
 subsection "Abstract functions"
 
 lemma typing_mono_app_cogent_absfun:
-  "\<lbrakk>proc_ctx_wellformed \<Xi>'; \<Xi>' f = ([], a, b)\<rbrakk> \<Longrightarrow> \<Xi>', [], [option.Some a] \<turnstile> App (AFun f []) (Var 0) : b"
+  "\<lbrakk>proc_ctx_wellformed \<Xi>'; \<Xi>' f = (0, [],{}, a, b)\<rbrakk> \<Longrightarrow> 
+   \<Xi>', 0, [], {}, [option.Some a] \<turnstile> App (AFun f [] []) (Var 0) : b"
   apply (unfold  proc_ctx_wellformed_def)
   apply (erule_tac x = f in allE; clarsimp)
-  apply (rule typing_app[where x = a and y = b and ?\<Gamma>1.0 = "[option.None]" and ?\<Gamma>2.0 = "[option.Some a]"]; simp?)
+  apply (rule typing_app[where x = a and y = b and 
+          ?\<Gamma>1.0 = "[option.None]" and ?\<Gamma>2.0 = "[option.Some a]"]; simp?)
     apply (clarsimp simp: split_conv_all_nth)
     apply (rule right; simp)
-   apply (rule typing_afun[where ts = "[]", OF _ _ _ _]; (simp add: Cogent.empty_def weakening_conv_all_nth)?)
-    apply clarsimp
-   apply (rule none)
+   apply (rule typing_afun[where ts = "[]"]; (simp add: Cogent.empty_def weakening_conv_all_nth)?)
+   apply (rule none, simp, simp add: subst_wellformed_nothing)
   apply (rule typing_var; simp add: Cogent.empty_def weakening_conv_all_nth)
   apply (rule keep; simp)
   done
 
 lemma typing_mono_afun_cogent_absfun:
-  "\<lbrakk>proc_ctx_wellformed \<Xi>'; \<Xi>' f = ([], a, b)\<rbrakk> \<Longrightarrow> \<Xi>', [], [option.None] \<turnstile> AFun f [] : TFun a b"
+  "\<lbrakk>proc_ctx_wellformed \<Xi>'; \<Xi>' f = (0, [], {}, a, b)\<rbrakk> \<Longrightarrow> 
+   \<Xi>', 0, [], {}, [option.None] \<turnstile> AFun f [] []: TFun a b"
   apply (unfold  proc_ctx_wellformed_def)
   apply (erule_tac x = f in allE; clarsimp)
-  apply (rule typing_afun[where ts = "[]", OF _ _ _ _]; (simp add: Cogent.empty_def weakening_conv_all_nth)?)
-   apply clarsimp
-  apply (rule none)
+  apply (rule typing_afun[where ts = "[]"]; 
+        (simp add: Cogent.empty_def weakening_conv_all_nth)?)
+    apply (rule none, simp, simp add: subst_wellformed_nothing)
   done
 
 lemma typing_mono_afun_imp_appafun:
-  "\<Xi>', [], [option.None] \<turnstile> AFun f [] : TFun a b \<Longrightarrow> \<Xi>', [], [option.Some a] \<turnstile> App (AFun f []) (Var 0) : b"
+  "\<Xi>', 0, [], {}, [option.None] \<turnstile> AFun f [] []: TFun a b \<Longrightarrow> 
+   \<Xi>', 0, [], {}, [option.Some a] \<turnstile> App (AFun f [] []) (Var 0) : b"
   apply (frule typing_to_wellformed(1))
   apply (rule typing_app[where x = a and y = b and ?\<Gamma>1.0 = "[option.None]" and ?\<Gamma>2.0 = "[option.Some a]"]; simp?)
    apply (clarsimp simp: split_conv_all_nth)
@@ -78,6 +88,7 @@ fun no_tvars
 "no_tvars TUnit = True" |
 "no_tvars (TVar _) = False" |
 "no_tvars (TVarBang _) = False" |
+"no_tvars (TCustomNum v) = True" |
 "no_tvars (TProduct a b) = (if no_tvars a then no_tvars b else False)" |
 "no_tvars (TFun a b) = (if no_tvars a then no_tvars b else False)" |
 "no_tvars (TCon n a b) = (find (\<lambda>x. \<not>x) (map no_tvars a) = option.None)" |
@@ -88,6 +99,7 @@ fun no_tfun
   where
 "no_tfun (TPrim _) = True" |
 "no_tfun TUnit = True" |
+"no_tfun (TCustomNum v) = True" |
 "no_tfun (TVar _) = undefined" |
 "no_tfun (TVarBang _) = undefined" |
 "no_tfun (TProduct a b) = (if no_tfun a then no_tfun b else False)" |
@@ -102,6 +114,7 @@ fun no_tcon
 "no_tcon TUnit = True" |
 "no_tcon (TVar _) = undefined" |
 "no_tcon (TVarBang _) = undefined" |
+"no_tcon (TCustomNum v) = True" |
 "no_tcon (TProduct a b) = (if no_tcon a then no_tcon b else False)" |
 "no_tcon (TFun a b) = (if no_tcon a then no_tcon b else False)" |
 "no_tcon (TCon n a b) = False" |
@@ -112,6 +125,7 @@ fun no_theap
   where
 "no_theap (TPrim _) = True" |
 "no_theap TUnit = True" |
+"no_theap (TCustomNum v) = True" |
 "no_theap (TVar _) = undefined" |
 "no_theap (TVarBang _) = undefined" |
 "no_theap (TProduct a b) = (if no_theap a then no_theap b else False)" |
@@ -124,6 +138,7 @@ fun no_taken
   where
 "no_taken (TPrim _) = True" |
 "no_taken TUnit = True" |
+"no_taken (TCustomNum v) = True" |
 "no_taken (TVar _) = undefined" |
 "no_taken (TVarBang _) = undefined" |
 "no_taken (TProduct a b) = (if no_taken a then no_taken b else False)" |
@@ -159,7 +174,7 @@ lemma no_heap_all_kinding_fn:
   done
 
 lemma no_heap_all_kind:
-  "\<lbrakk>no_tvars t; no_theap t; K \<turnstile> t wellformed\<rbrakk> \<Longrightarrow> K \<turnstile> t :\<kappa> UNIV"
+  "\<lbrakk>no_tvars t; no_theap t; 0, K, {} \<turnstile> t wellformed\<rbrakk> \<Longrightarrow> 0, K, {}\<turnstile> t :\<kappa> UNIV"
   apply (rule kindingI; simp add: no_heap_all_kinding_fn)
   done
 
